need to figure out the inv for magic_mul

NativeTypes.dfy
@@ -78,4 +78,11 @@ module NativeTypes {
     {
         if x > y then y else x
     }
+
+    function method lh_64(x: uint64) : (r: uint32)
+
+    function method uh_64(x: uint64) : (r: uint32)
+
+    lemma upper_lower_halves_64_lemma(x: uint64) 
+      ensures uh_64(x)  as int * (UINT32_MAX as int + 1) + lh_64(x) as int == x as int;
 }
